compiler/backend/data_to_wordScript.sml
@@ -2305,6 +2305,16 @@ val compile_def = Define `
     let p = stubs (:α) data_conf ++ MAP (compile_part data_conf) prog in
       word_to_word$compile word_conf (asm_conf:'a asm_config) p`;
 
+Definition compile_to_word_def:
+  compile_to_word data_conf asm_conf prog =
+    let data_conf = (data_conf with
+                      <| has_fp_ops := (1 < asm_conf.fp_reg_count);
+                         has_fp_tern := (asm_conf.ISA = ARMv7 /\
+                                         2 < asm_conf.fp_reg_count) |>)
+    in
+      stubs (:α) data_conf ++ MAP (compile_part data_conf) prog
+End
+
 (* compute bignum call graph *)
 
 val th_FF = EVAL ``full_call_graph AnyArith_location
